more loop invariant automation

refinedVST/typing/bytes.v
@@ -273,13 +273,30 @@ Section uninit.
   Global Existing Instance type_read_move_copy_inst | 70. *)
 
   Definition ty_own_var_uninit f x : assert :=
-    match list_to_map(M := gmap ident Ctypes.type) (f.(fn_params) ++ f.(fn_temps)) !! x with
-    | Some cty => env.temp x Vundef
-    | None => match list_to_map(M := gmap ident Ctypes.type) f.(fn_vars) !! x with
-              | Some cty => ∃ b, env.lvar x cty b ∗ ⎡(b, Ptrofs.zero) ◁ₗ uninit cty⎤
-              | None => False
-              end
-    end.
+    (∃ cty, <affine> ⌜(x, cty) ∈ f.(fn_params) ++ f.(fn_temps)⌝ ∗ ∃ v, env.temp x v) ∨
+    (∃ cty, <affine> ⌜(x, cty) ∈ f.(fn_vars)⌝ ∗ ∃ b, env.lvar x cty b ∗ ⎡(b, Ptrofs.zero) ◁ₗ uninit cty⎤).
+
+  Lemma simplify_goal_ty_own_var_uninit_temp f x cty
+    `{!TCElemOf (x, cty) (f.(fn_params) ++ f.(fn_temps))} T:
+    (∃ v, env.temp x v ∗ T) ⊢ simplify_goal (ty_own_var_uninit f x) T.
+  Proof.
+    rewrite /ty_own_var_uninit; iIntros "(% & ? & $)".
+    iLeft; iFrame.
+    iPureIntro; eexists; by apply TCElemOf_inv.
+  Qed.
+  Definition simplify_goal_ty_own_var_uninit_temp_inst := [instance simplify_goal_ty_own_var_uninit_temp with 10%N].
+  Global Existing Instance simplify_goal_ty_own_var_uninit_temp_inst.
+
+  Lemma simplify_goal_ty_own_var_uninit_local f x cty
+    `{!TCElemOf (x, cty) (f.(fn_vars))} T:
+    (∃ b, env.lvar x cty b ∗ ⎡(b, Ptrofs.zero) ◁ₗ uninit cty⎤ ∗ T) ⊢ simplify_goal (ty_own_var_uninit f x) T.
+  Proof.
+    rewrite /ty_own_var_uninit; iIntros "(% & ? & ? & $)".
+    iRight; iFrame.
+    iPureIntro; by apply TCElemOf_inv.
+  Qed.
+  Definition simplify_goal_ty_own_var_uninit_local_inst := [instance simplify_goal_ty_own_var_uninit_local with 10%N].
+  Global Existing Instance simplify_goal_ty_own_var_uninit_local_inst.
 
 End uninit.
 
